Add work

src/Env.v
@@ -13,9 +13,9 @@ Module Env (P : PAT).
   .
 
   Inductive binding : Type :=
-  | BindTname : binding
+  | BindTName : binding
   | BindCon   : data -> type -> tname -> binding
-  | BindTvar  : kind -> binding
+  | BindTVar  : kind -> binding
   | BindVar   : type -> binding
   | BindMatch : match_assum -> binding
   .
@@ -24,13 +24,13 @@ Module Env (P : PAT).
 
   Definition empty_env : env := nil.
 
-  Definition is_tname (b : binding) : Prop := match b with BindTname => True | _ => False end.
+  Definition is_tname (b : binding) : Prop := match b with BindTName => True | _ => False end.
   Definition tnames   (Gamma : env) : env := filter is_tname Gamma.
 
   Definition is_con (b : binding) : Prop := match b with BindCon _ _ _ => True | _ => False end.
   Definition cons   (Gamma : env) : env := filter is_con Gamma.
 
-  Definition is_tvar (b : binding) : Prop := match b with BindTvar _ => True | _ => False end.
+  Definition is_tvar (b : binding) : Prop := match b with BindTVar _ => True | _ => False end.
   Definition tvars   (Gamma : env) : env := filter is_tvar Gamma.
 
   Definition is_var (b : binding) : Prop := match b with BindVar _ => True | _ => False end.
@@ -42,16 +42,35 @@ Module Env (P : PAT).
   Definition binds (n : nat) (b : binding) (Gamma : env) : Prop := Nth n Gamma b.
 
   Definition tname_in (T : tname) (Gamma : env) : Prop :=
-    binds T BindTname (tnames Gamma).
+    binds T BindTName (tnames Gamma).
 
   Definition con_in (K : con) (d : data) (ty : type) (T : tname) (Gamma : env) : Prop :=
     binds K (BindCon d ty T) (cons Gamma).
 
   Definition tvar_in (tv : tvar) (k : kind) (Gamma : env) : Prop :=
-    binds tv (BindTvar k) (tvars Gamma).
+    binds tv (BindTVar k) (tvars Gamma).
 
   Definition var_in (v : var) (ty : type) (Gamma : env) : Prop :=
     binds v (BindVar ty) (vars Gamma).
+
+
+  Definition freshen_after (Gamma : env) : env :=
+    map
+      (fun b =>
+         match b with
+         | BindVar ty => BindVar (ty_freshen ty 0)
+         | _          => b
+         end)
+      Gamma.
+
+  Definition freshen_before (Gamma : env) : env :=
+    fold_right
+      (fun b Gamma' =>
+         match b with
+         | BindVar ty => BindVar (ty_freshen ty (length Gamma'))
+         | _          => b
+         end :: Gamma')
+      nil Gamma.
 
 
   Create HintDb rew_env.
@@ -75,21 +94,6 @@ Module Env (P : PAT).
   Tactic Notation "rew_env" "*" "in" hyp(H) :=
     rew_env in H; auto_star.
 
-
-  Lemma vars_app : forall G1 G2, vars (G1 ++ G2) = vars G1 ++ vars G2.
-  Proof. intros. unfold vars. rew_listx~. Qed.
-
-  Lemma vars_cons : forall Gamma b,
-      vars (b :: Gamma) =
-        match b with
-        | BindVar _ => b :: vars Gamma
-        | _         => vars Gamma
-        end.
-  Proof. intros ; destruct b ; unfolds ; unfolds is_var ; rew_listx ; case_if*. Qed.
-
-  #[export]
-  Hint Rewrite vars_app vars_cons : rew_env.
-
   Lemma binds_app_middle_inv :
     forall x y1 y2 G1 G2,
       binds x y1 (G1 ++ y2 :: G2) ->
@@ -105,5 +109,79 @@ Module Env (P : PAT).
       { left*. }
       { right. split*. simple_math. applys_eq (>> Nth_app_r G1 in_G2). nat_math. } }
   Qed.
+
+  Lemma binds_weaken :
+    forall x y y' G1 G2,
+      binds x y (G1 ++ G2) ->
+      x < length G1 /\ binds x y (G1 ++ y' :: G2)
+      \/ x >= length G1 /\ binds (S x) y (G1 ++ y' :: G2).
+  Proof.
+  Admitted.
+
+  (* Lemma binds_freshen : *)
+  (*   forall x ty ty' G1 G2, *)
+  (*     binds x (BindVar ty) (G1 ++ G2) -> *)
+  (*     binds x (BindVar (ty)) (G1 ++ G2) -> *)
+  (*     x < length G1 /\ binds x y (G1 ++ y' :: G2) *)
+  (*     \/ x >= length G1 /\ binds (S x) y (G1 ++ y' :: G2). *)
+  (* Proof. *)
+  (* Admitted. *)
+
+  Lemma tnames_app : forall G1 G2, tnames (G1 ++ G2) = tnames G1 ++ tnames G2.
+  Proof. intros. unfold tnames. rew_listx~. Qed.
+
+  Lemma tnames_cons : forall Gamma b,
+      tnames (b :: Gamma) =
+        match b with
+        | BindTName => b :: tnames Gamma
+        | _         => tnames Gamma
+        end.
+  Proof. intros ; destruct b ; unfolds ; unfolds is_tname ; rew_listx ; case_if*. Qed.
+
+  #[export]
+  Hint Rewrite tnames_app tnames_cons : rew_env.
+
+  Lemma cons_app : forall G1 G2, cons (G1 ++ G2) = cons G1 ++ cons G2.
+  Proof. intros. unfold cons. rew_listx~. Qed.
+
+  Lemma cons_cons : forall Gamma b,
+      cons (b :: Gamma) =
+        match b with
+        | BindCon _ _ _ => b :: cons Gamma
+        | _             => cons Gamma
+        end.
+  Proof. intros ; destruct b ; unfolds ; unfolds is_con ; rew_listx ; case_if*. Qed.
+
+  #[export]
+  Hint Rewrite cons_app cons_cons : rew_env.
+
+  Lemma tvars_app : forall G1 G2, tvars (G1 ++ G2) = tvars G1 ++ tvars G2.
+  Proof. intros. unfold tvars. rew_listx~. Qed.
+
+  Lemma tvars_cons : forall Gamma b,
+      tvars (b :: Gamma) =
+        match b with
+        | BindTVar _ => b :: tvars Gamma
+        | _          => tvars Gamma
+        end.
+  Proof. intros ; destruct b ; unfolds ; unfolds is_tvar ; rew_listx ; case_if*. Qed.
+
+  #[export]
+  Hint Rewrite tvars_app tvars_cons : rew_env.
+
+
+  Lemma vars_app : forall G1 G2, vars (G1 ++ G2) = vars G1 ++ vars G2.
+  Proof. intros. unfold vars. rew_listx~. Qed.
+
+  Lemma vars_cons : forall Gamma b,
+      vars (b :: Gamma) =
+        match b with
+        | BindVar _ => b :: vars Gamma
+        | _         => vars Gamma
+        end.
+  Proof. intros ; destruct b ; unfolds ; unfolds is_var ; rew_listx ; case_if*. Qed.
+
+  #[export]
+  Hint Rewrite vars_app vars_cons : rew_env.
 
 End Env.
