src/Typing.v
@@ -1,5 +1,7 @@
 From MCore Require Import Syntax Env Tactics.
-From TLC Require Import LibString LibList LibSet.
+From TLC Require Import LibString LibNat LibList LibSet.
+
+Open Scope nat_scope.
 
 Module Typing (P : PAT).
   Module E := Env P.
@@ -47,7 +49,7 @@ Module Typing (P : PAT).
         ok_type Gamma ty2 KiType ->
         ok_type Gamma (TyArr ty1 ty2) KiType
     | TyAll' : forall {Gamma : env} {k : kind} {ty : type},
-        ok_type (BindTvar k :: Gamma) (ty_open ty 0 0) KiType ->
+        ok_type (BindTVar k :: Gamma) (ty_open ty 0 0) KiType ->
         ok_type Gamma (TyAll k ty) KiType
     (* | TyProd' : forall {Gamma : env} {ty1 ty2 : type}, *)
     (*     ok_type Gamma ty1 KiType -> *)
@@ -75,7 +77,7 @@ Module Typing (P : PAT).
 
     Inductive ok_env : env -> Prop :=
     | EnvEmpty : ok_env empty_env
-    | EnvTname : forall Gamma, ok_env Gamma -> ok_env (BindTname :: Gamma)
+    | EnvTName : forall Gamma, ok_env Gamma -> ok_env (BindTName :: Gamma)
     | EnvCon   :
       forall Gamma d ty T,
         ok_env Gamma ->
@@ -83,10 +85,10 @@ Module Typing (P : PAT).
         ok_type Gamma ty KiType ->
         tname_in T (tnames Gamma) ->
         ok_env (BindCon d ty T :: Gamma)
-    | EnvTvar : forall Gamma k,
+    | EnvTVar : forall Gamma k,
         ok_env Gamma ->
         ok_kind Gamma k ->
-        ok_env (BindTvar k :: Gamma)
+        ok_env (BindTVar k :: Gamma)
     | EnvVar : forall Gamma ty,
         ok_env Gamma ->
         ok_type Gamma ty KiType ->
@@ -113,7 +115,8 @@ Module Typing (P : PAT).
         ok_term Gamma (TmApp t1 t2) ty2
     | TmTyLam' : forall {Gamma : env} {k : kind} {ty : type} {t : term},
         ok_kind Gamma k ->
-        ok_term (BindTvar k :: Gamma) (tm_ty_open t 0 0) (ty_open ty 0 0) ->
+        ok_term (BindTVar k :: freshen_after Gamma)
+                (tm_ty_open t 0 0) (ty_open ty 0 0) ->
         ok_term Gamma (TmTyLam k t) (TyAll k ty)
     | TmTyApp' : forall {Gamma : env} {k : kind} {ty1 ty2 : type} {t : term},
         ok_term Gamma t (TyAll k ty1) ->
@@ -204,6 +207,8 @@ Module Typing (P : PAT).
         ok_type Gamma ty k ->
         ty_lc ty.
     Proof. introv tykind. induction* tykind. Qed.
+    #[export]
+     Hint Resolve ok_type_lct : mcore.
 
     Lemma ok_env_type :
       forall G1 G2 ty,
@@ -229,109 +234,156 @@ Module Typing (P : PAT).
       forall Gamma t ty,
         ok_term Gamma t ty ->
         ty_lc ty.
-    Proof.
+    Proof with eauto using ty_lc_fsubst with mcore.
       introv ttype. induction* ttype.
       { Case "TmVar". apply* ok_env_lct. }
-      { Case "TmLam". constructor*. apply* ok_type_lct. }
       { Case "TmApp". inverts* IHttype1. }
       { Case "TmTyApp".
-        inverts* IHttype.
         rewrite ty_bsubst_close_open with (x := 0).
-        apply ty_defreshen_lc. apply* ty_lc_fsubst. apply ty_freshen_lc. apply* ok_type_lct. }
+        inverts IHttype... }
     Qed.
-
     #[export]
-     Hint Extern 1 (ty_lc ?ty) =>
-      match goal with
-      | H: ok_term ?Gamma ?t ty |- _ => apply (ok_term_lct Gamma t ty)
-      | H: ok_type ?Gamma ty ?k |- _ => apply (ok_type_lct Gamma ty k)
-      end
-      : mcore.
-
-    #[export]
-     Hint Extern 1 (ty_lc (ty_freshen ?ty _)) =>
-      match goal with
-      | H: ok_term _ _ ty |- _ => apply ty_freshen_lc
-      | H: ok_type _ ty _ |- _ => apply ty_freshen_lc
-      end
-      : mcore.
+     Hint Resolve ok_term_lct : mcore.
 
     Lemma ok_term_lc :
       forall Gamma t ty,
         ok_term Gamma t ty ->
         tm_lc t.
     Proof. introv ttype. induction* ttype. Qed.
-
     #[export]
-     Hint Extern 1 (tm_lc ?t) =>
-      match goal with
-      | H: ok_term ?Gamma t ?ty |- _ => apply (ok_term_lc Gamma t ty)
-      end
-      : mcore.
+     Hint Resolve ok_term_lc : mcore.
 
-    #[export]
-     Hint Extern 1 (tm_lc (tm_freshen ?t _)) =>
-      match goal with
-      | H: ok_term _ t _ |- _ => apply tm_freshen_lc
-      end
-      : mcore.
+    Lemma ok_data_weaken_var :
+      forall G1 G2 ty' d,
+        ok_data (G1 ++ G2) d ->
+        ok_data (G1 ++ BindVar ty' :: G2) d.
+    Proof. introv Hd. unfolds ok_data. rew_env* in *. Qed.
+
+    Lemma ok_kind_weaken_var :
+      forall G1 G2 ty' k,
+        ok_kind (G1 ++ G2) k ->
+        ok_kind (G1 ++ BindVar ty' :: G2) k.
+    Proof. introv Hk. induction* Hk. Qed.
+
+    Lemma ok_kind_weaken_tvar :
+      forall G1 G2 k' k,
+        ok_kind (G1 ++ G2) k ->
+        ok_kind (G1 ++ BindTVar k' :: G2) k.
+    Proof. introv Hk. induction* Hk. Qed.
+
+    Lemma ok_type_weaken_var :
+      forall G1 G2 ty ty' k,
+        ok_type (G1 ++ G2) ty k ->
+        ok_type (G1 ++ BindVar ty' :: G2) ty k.
+    Proof.
+      introv Hty.
+      remember (G1 ++ G2) as Gamma eqn:HGamma.
+      gen G1.
+      induction Hty ; intros ; subst*.
+      { Case "TyFVar". constructor. unfolds tvar_in. rew_env* in *. }
+      { Case "TyAll". constructor. applys IHHty (BindTVar k :: G1). rew_list*. }
+    Qed.
+
+    Lemma ok_type_weaken_tvar :
+      forall G1 G2 x ty k' k,
+        x = length (tvars G1) ->
+        ok_type (G1 ++ G2) ty k ->
+        ok_type (freshen_before G1 ++ BindTVar k' :: freshen_after G2) (ty_freshen ty x) k.
+    Proof.
+      introv Heq Hty.
+      remember (G1 ++ G2) as Gamma eqn:HGamma.
+      gen G1 x.
+      induction Hty ; intros ; subst*.
+      { Case "TyFVar". unfold ty_freshen. simple_math. admit. admit. }
+      Admitted.
+
+    Lemma ok_term_weaken_var :
+      forall G1 G2 x t ty ty',
+        x = length (vars G1) ->
+        ok_term (G1 ++ G2) t ty ->
+        ok_env  (G1 ++ BindVar ty' :: G2) ->
+        ok_term (G1 ++ BindVar ty' :: G2) (tm_freshen t x) ty.
+    Proof with rew_env ; rew_list ; eauto using ok_kind_weaken_var, ok_type_weaken_var with mcore.
+    Admitted.
+    (*   introv Heq ttype. *)
+    (*   remember (G1 ++ G2) as Gamma eqn:HGamma. *)
+    (*   gen G1 x. *)
+    (*   induction ttype ; intros ; subst ; simpls... *)
+    (*   { Case "TmFVar". unfolds var_in. rew_env in *. *)
+    (*     forwards [ (Hlt & Hvar) | (Hge & Hvar) ] *)
+    (*       : binds_weaken ; simple_math ; constructor ; unfolds var_in... } *)
+    (*   { Case "TmLam". constructor... rewrite* tm_open_freshen_comm. *)
+    (*     applys IHttype (BindVar ty1 :: G1)... } *)
+    (*   { Case "TmTyLam". constructor... rewrite* tm_ty_open_freshen_comm. *)
+    (*     apply (IHttype (BindTVar k :: (map_vars (fun ty'0 => ty_freshen ty'0 0) G1)))... } *)
+    (* Qed. *)
+
+    (* Lemma ok_env_freshen : *)
+    (*   forall G1 G2 k, *)
+    (*     ok_env (G1 ++ G2) -> *)
+    (*     ok_kind G2 k -> *)
+    (*     ok_env (map_vars ty_freshen G1 ++ BindTVar k :: G2). *)
+    (* Proof. *)
+    (*   introv Henv Hk. *)
+    (*   induction G1. *)
+    (*   Admitted. *)
+    (*   { Case "nil". unfold env_freshen. rew_listx*. } *)
+    (*   { Case "cons". unfold env_freshen. rew_listx. } *)
+    (* Admitted. *)
+
+    Lemma ok_term_weaken_tvar :
+      forall G1 G2 x t ty k,
+        x = length (tvars G1) ->
+        ok_term (G1 ++ G2) t ty ->
+        ok_env  (freshen_before G1 ++ BindTVar k :: G2) ->
+        ok_term (freshen_before G1 ++ BindTVar k :: G2) (tm_ty_freshen t x) (ty_freshen ty x).
+    Proof with rew_env ; rew_list ; eauto using ok_kind_weaken_tvar, ok_type_weaken_tvar with mcore.
+      introv Heq ttype.
+      remember (G1 ++ G2) as Gamma eqn:HGamma.
+      gen G1 x.
+      induction ttype ; intros ; subst ; simpls*.
+      Admitted.
+      (* { Case "TmFVar". constructor*. unfolds var_in. rew_env in *... } *)
+      (* { Case "TmLam". constructor. unfolds var_in. rew_env in *... } *)
 
     Lemma ok_data_strengthen_var :
       forall G1 G2 ty' d,
         ok_data (G1 ++ BindVar ty' :: G2) d ->
         ok_data (G1 ++ G2) d.
-    Proof. Admitted.
+    Proof. introv Hd. unfolds ok_data. rew_env* in *. Qed.
 
     Lemma ok_kind_strengthen_var :
       forall G1 G2 ty' k,
         ok_kind (G1 ++ BindVar ty' :: G2) k ->
         ok_kind (G1 ++ G2) k.
-    Proof. Admitted.
+    Proof. introv Hk. induction* Hk. Qed.
 
     Lemma ok_type_strengthen_var :
       forall G1 G2 ty' ty k,
         ok_type (G1 ++ BindVar ty' :: G2) ty k ->
         ok_type (G1 ++ G2) ty k.
-    Proof. Admitted.
+    Proof.
+      introv Hty.
+      remember (G1 ++ BindVar ty' :: G2) as Gamma eqn:HGamma.
+      gen G1.
+      induction Hty ; intros ; subst*.
+      { Case "TyFVar". constructor. unfolds tvar_in. rew_env* in *. }
+      { Case "TyAll". constructor. applys IHHty (BindTVar k :: G1). rew_list*. }
+    Qed.
 
     Lemma ok_env_strengthen_var :
       forall G1 G2 ty,
         ok_env (G1 ++ BindVar ty :: G2) ->
         ok_env (G1 ++ G2).
-    Proof. Admitted.
-    (*   introv Henv. induction* G1 ; rew_list in *. inverts* Henv. *)
-    (*   destruct* a ; inverts* Henv. constructor*. *)
-    (*   apply* ok_data_strengthen_var. apply* ok_type_strengthen_var. unfolds tnames. rew_listx in *. *)
-    (*   unfold is_tname in *. rew_env* in *. *)
-    (*   constructor. apply* IHG1. apply* ok_kind_strengthen_var. *)
-    (*   constructor. apply* IHG1. apply* ok_type_strengthen_var. *)
-    (* Qed. *)
+    Proof with eauto using ok_data_strengthen_var, ok_kind_strengthen_var, ok_type_strengthen_var.
+      introv Henv ; induction* G1 ; rew_list in * ; inverts* Henv ; constructor ; rew_env in *...
+    Qed.
 
-    Lemma tm_freshen_preservation :
-      forall Gamma t ty ty',
+    Lemma ok_term_ok_env :
+      forall Gamma t ty,
         ok_term Gamma t ty ->
-        ok_term (BindVar ty' :: Gamma) (tm_freshen t 0) ty.
-    Proof. Admitted.
-
-    #[export]
-     Hint Extern 1 (ok_term _ (tm_freshen ?t _) _) =>
-      match goal with
-      | H: ok_term _ t _ |- _ => apply tm_freshen_preservation
-      end
-      : mcore.
-
-    Lemma tm_ty_freshen_preservation :
-      forall Gamma t ty k,
-        ok_term Gamma t ty ->
-        ok_term (BindTvar k :: Gamma) (tm_ty_freshen t 0) ty.
-    Proof. Admitted.
-
-    #[export]
-     Hint Extern 1 (ok_term _ (tm_ty_freshen ?t _) _) =>
-      match goal with
-      | H: ok_term _ t _ |- _ => apply tm_ty_freshen_preservation
-      end
-      : mcore.
+        ok_env Gamma.
+    Proof. introv ttype ; induction* ttype ; inverts* IHttype. Admitted.
 
     Lemma tm_close_preservation :
       forall G1 G2 x t t' ty1 ty2,
@@ -340,24 +392,28 @@ Module Typing (P : PAT).
         ok_term (G1 ++ G2) t' ty1 ->
         ok_term (G1 ++ G2) (tm_close t x t') ty2.
     Proof with rew_env ; rew_list
-    ; eauto using ok_env_strengthen_var, ok_kind_strengthen_var, ok_type_strengthen_var with mcore.
+      ; eauto using ok_term_ok_env, ok_kind_strengthen_var, ok_type_strengthen_var, ok_env_strengthen_var
+        with mcore.
       introv Heq ttype. unfolds tm_close.
       remember (G1 ++ BindVar ty1 :: G2) as Gamma eqn:HGamma.
-      gen t' G1 x.
+      gen ty1 t' G1 x.
       induction ttype ; intros ; subst ; simpls...
       { Case "TmFVar". unfolds var_in. rew_env in *.
-        forwards* [ (Hlt & Hvar') | [ (Heq1 & Heq2) | (Hgt & Hvar') ] ]
+        forwards [ (Hlt & Hvar') | [ (Heq1 & Heq2) | (Hgt & Hvar') ] ]
           : binds_app_middle_inv ; subst ; simple_math ; try (constructor ; unfolds var_in)...
         inverts* Heq2. rewrite* tm_defreshen_freshen. }
       { Case "TmLam". constructor... folds (tm_close t (length (vars G1)) t').
-        rewrite* tm_open_close_comm. applys IHttype (BindVar ty0 :: G1)... }
-      { Case "TmTyLam".  constructor... folds (tm_close t (length (vars G1)) t').
-        rewrite* tm_ty_open_close_comm. applys IHttype (BindTvar k :: G1)... }
+        rewrite* tm_open_close_comm. applys IHttype (BindVar ty1 :: G1)...
+        applys_eq (ok_term_weaken_var empty_env)... }
+      { Case "TmTyLam". constructor... folds (tm_close t (length (vars G1)) t').
+        rewrite* tm_ty_open_close_comm. unfolds freshen_after. rew_listx in *.
+        apply (IHttype (ty_freshen ty1 0) (tm_ty_freshen t' 0) (BindTVar k :: freshen_after G1)).
+        applys_eq (ok_term_weaken_tvar empty_env)... }
     Qed.
 
     Lemma tm_ty_close_preservation :
       forall Gamma t ty ty' k,
-        ok_term (BindTvar k :: Gamma) (tm_ty_open t 0 0) (ty_open ty 0 0) ->
+        ok_term (BindTVar k :: Gamma) (tm_ty_open t 0 0) (ty_open ty 0 0) ->
         ok_type Gamma ty' k ->
         ok_term Gamma (tm_ty_bsubst t 0 ty') (ty_bsubst ty 0 ty').
     Proof. Admitted.
